Commented and cleaned ProbabilismHoare

ProbabilismHoare.fst
@@ -14,78 +14,73 @@ open FStar.List.Tot
 open FStar.Tactics
 open FStar.FunctionalExtensionality
 
-(* let tmp () : Lemma(exists (f:prop -> bool). f True = true /\ f False = false) =
-assert(~ (True == False));
-  assert_by_tactic(exists (f:bool -> bool). f true = true /\ f false = false)
-(fun _ ->
-smt();
-dump "tmp";
-admit_all());
-admit() *)
-
+// Non-negative reals (pr like probability is a slight misnomer
+// because we do not upper bound it by 1)
 let pr = r:real{r >=. zero}
-let prob_pre = pr
-let prob_post (a:Type) = a -> Tot pr
-let prob_wp (a:Type) = prob_pre ^-> prob_post a ^-> prop
 
+// Post-condition type
+let prob_post (a:Type) = a -> Tot pr
+
+// Weakest precondition type
+// TODO: maybe add suitable monotonicity constraints as refinement
+let prob_wp (a:Type) = pr -> prob_post a -> Type0
+
+// Models a probability distribution, basically (f:a -> pr){sum <= 1}
 assume type distribution (a:Type) : Type
 
+// Distribution that gives probability 1 to x
 assume val point_distribution (#a:Type) (x:a) : distribution a
 
+// Uniform distribution on x (must be a non-empty list)
 assume val uniform_distribution (#a:Type) (x:list a{Cons? x}) : distribution a
 
-let prob_wp_eqI #a (wp1 wp2: prob_wp a) :
-    Lemma (requires (forall pre post. wp1 pre post == wp2 pre post))
-          (ensures (wp1 == wp2)) = 
-    assert (forall pre. feq (wp1 pre) (wp2 pre));
-    assert (feq wp1 wp2);
-    assert (wp1 == wp2)
-
+// Representation type for PROB effect.
+// "prob a w" is the type of distributions f over a that satisfy the wp w.
+// (I.e., they satisfy "forall pre post, w pre post -> sum_{x:a} f(x)post(x) >= pre.)
+// TODO: A refinement has to be added with that condition
 let prob a (w:prob_wp a): Tot Type0 =
   distribution a // TODO: require w to hold
 
-let b2p (b: bool) : prop = b == true
-let t2p (t: Type0) : prop = t
+// let b2p (b: bool) : prop = b == true
 
+//let t2p (t: Type0) : prop = t
+
+// Wp corresponding to "prob_return x"
 let prob_wreturn #a x : prob_wp a = 
-    on _ (fun (pre:prob_pre) -> on _ (fun (post:prob_post a) -> b2p (pre <=. post x)))
+    (fun (pre:pr) -> (fun (post:prob_post a) -> pre <=. post x))
 
+// Semantics of "return x"
 let prob_return a (x:a) : prob a (prob_wreturn x) = 
   point_distribution x
 
+// Wp corresponding to "let x = p1 in p2 x", given the wps for p1, p2
 let prob_wbind #a #b (w1:prob_wp a) (w2:a -> prob_wp b) : prob_wp b = 
-    on _ (fun (pre:prob_pre) -> on _ (fun (post:prob_post b) ->
+    (fun (pre:pr) -> (fun (post:prob_post b) ->
       exists (mid:prob_post a). w1 pre mid /\ (forall (x:a). w2 x (mid x) post)))
 
-let prob_bind a b (w1:prob_wp a) (w2:a -> prob_wp b)
-      (f: prob a w1) (g: (x:a -> prob b (w2 x))) : prob b (prob_wbind w1 w2) =
-   admit()   
+// Semantics of "let x = p1 in p2 x"
+assume val prob_bind (a b:Type) (w1:prob_wp a) (w2:a -> prob_wp b)
+      (f: prob a w1) (g: (x:a -> prob b (w2 x))) : prob b (prob_wbind w1 w2)
 
 let stronger #a (w1 w2:prob_wp a) = forall post pre. w2 post pre ==> w1 post pre
 
-let prob_wp_stronger_eq #a (w1 w2:prob_wp a) :
-    Lemma (requires w1 `stronger` w2 /\ w2 `stronger` w1)
-    	  (ensures w1 == w2) = 
-    assert (w1 == w2) by (
-apply_lemma (`prob_wp_eqI);
-let pre = forall_intro_as "pre" in
-let post = forall_intro_as "post" in
-let _ = pose_lemma (`FStar.PropositionalExtensionality.axiom) in
-dump "";
-admit_all()
-)
-
+// Weakening in the PROB effect: takes "f:prob a w1" and returns the same f with a different type "prob a w2",
+// assuming w2 is a weaker wp than w2
 let prob_subcomp a (w1 w2 : prob_wp a) (f:prob a w1) : 
-                 Pure (prob a w2) (requires w1 `prob_stronger` w2) (ensures (fun _ -> True)) =
+                 Pure (prob a w2) (requires w1 `stronger` w2) (ensures (fun _ -> True)) =
   f
 
+// Semantics of if-then-else in a probabilistic program.
+// Since the condition is a fixed boolean, this is quite trivial.
 let ite_prob a (#w1 #w2 : prob_wp a) (f: prob a w1) (g: prob a w2) (b: bool) : Type =
   prob a (if b then w1 else w2)
 
-// [@@allow_informative_binders] // Can we get rid of this and still have reifiable?
+// Defining the PROB effect. Representation type is prob, and the
+// effect is defined using the various specifications of the semantics
+// that we defined above.
 total
-//reifiable
-reflectable
+reifiable // Works here! (Doesn't work in ProbabilismWP because repr is "informative"
+reflectable // Means we can create a probabilistic function from an explicitly given distribution. See coin below.
 layered_effect { PROB : (a:Type) -> (wp:prob_wp a) -> Effect with 
   repr = prob;
   return = prob_return; 
@@ -94,186 +89,38 @@ layered_effect { PROB : (a:Type) -> (wp:prob_wp a) -> Effect with
   if_then_else = ite_prob
   }
 
-// assume val smallest : #a:Type -> (a->Type) -> (a->pr) -> pr
-
-// effect PTotal a (pre:prop) (post:a->prop) = PROB a (fun p -> smallest (fun x -> pre ==> post x) p)
-// effect PPartial a (pre:Type0) (post:a->Type0) = PROB a (fun p -> ? smallest (fun x -> pre ==> post x) p)
-
-
-(*
-I think the problem with the definition is the following:
-
-In a call such as "f x" where x:t is pure and f:t->PROB u, this
-desugars roughly to "bind_prob (lift_pure_prob x) f" lift_pure_prob x
-has an implicit #pwp that needs to be instantiated, but bind_prob does
-not put any constraint on the wp returned by lift_pure_prob, so there
-is no information how to instantiate #pwp. Hence "f x" fails (in many
-cases).
-
-Ideas:
-
-* Is there some way how to guide the insertion of implicits?
-
-* Can we define a function "list_pure_prob_wp : pure_wp a -> prob_wp
-  a" so that we do not need #pwp. Problem: this needs a function
-  "largest (real -> Type)" that is probably not implementable and
-  whose axiomatized existence might be unsound (allows to solve the
-  halting problem or equality on functions). largest could be
-  constrained to require that the input is a Dedekind cut, but it is
-  still not obvious that largest would be sound then. (Also, this
-  approach might not even be possible for quantum WPs because
-  Hermitian operators form an antilattice.)
-
-* Can we add type hints in a PROB function to indicate the wp's? 
-
-* Can we tell F* to avoid using the lifting in cases where it cancels
-  out anyway? (E.g., "bind_prob (lift_pure_prob x) f" could just be "f
-  x".
-
-* We can define prob_wp as a union type "Prob_WP of (prob_post ->
-  prob_pre) | Pure_WP of pure_wp". Then translating from PURE to PROB
-  is trivial. All other monadic transformations need to be adapted to
-  deal with the case distinction. (In particular subcomp must handle
-  comparison between PURE and PROB (in one direction only).)
-
-* Model reals as dedekind cuts
-
-* Model prob_wp a := prob_post a -> Type0. Intuition: (prob_wp a p)
-  holds iff expectation of p is >= 1.
-
-* Model prob_wp a := relation between pre/post-condition
-
-*)
-
+// Given PURE-wp wp, this returns the corresponding wp of the
+// probabilistic program.  I.e., if f:PURE wp, then "return f : PROB
+// (lift_pure_prob_wp wp)", roughly speaking.
 let lift_pure_prob_wp #a (wp:pure_wp a) : prob_wp a =
     fun pre post -> wp (fun x -> pre <=. post x)
 
+// Given pure program f, returns the corresponding probabilistic program "return f"
 let lift_pure_prob a (wp:pure_wp a) (f: eqtype_as_type unit -> PURE a wp) : 
-   prob a (lift_pure_prob_wp wp) =
-   assume False; // TODO
+   prob a (lift_pure_prob_wp wp) by (admit_all()) =
    point_distribution (f ())
    
 sub_effect PURE ~> PROB = lift_pure_prob
 
-// let hint a : squash(forall (y x:a). (forall post. post y ==> post x) ==> (x == y)) = admit()
+// Helper function. Constructs a wp in the Hoare-approach (type prob_wp above) from a wp in the wp-approach.
+let from_wp #a (wp: prob_post a -> pr) : prob_wp a = fun pre post -> pre <=. wp post
 
-// let hint_string () = hint string
-
-(* let average (l:list pr{Cons? l}) : pr =
-  assume False;
-  (fold_left (fun pr x -> pr +. x) zero l) /. of_int (length l)
-
-let pick #a (l:list a{Cons? l}) : PROB a (fun post -> average (map post l)) =
-  PROB?.reflect (uniform_distribution l) *)
-
-let simple_wp #a (wp: prob_post a -> pr) : prob_wp a = fun pre post -> pre <=. wp post
-
-let coin () : PROB bool (simple_wp (fun post -> (post true +. post false) /. two)) =
+// A basic function for writing probabilistic programs. Returns a random bool.
+// The type characterizes this.
+let coin () : PROB bool (from_wp (fun post -> (post true +. post false) /. two)) =
   PROB?.reflect (uniform_distribution [true;false])
 
 (**** TESTS *****)
 
-let test1 () : PROB bool (simple_wp (fun post -> (post true +. post false) /. two)) = coin ()
+// Some very simple tests (anything beyond that would probably need a simplifier like in ProbabilismWP).
+
+let test1 () : PROB bool (from_wp (fun post -> (post true +. post false) /. two)) = coin ()
 
 let test2 () : PROB bool (fun pre post -> False) = coin ()
 
-(* let return (#a) (x:a) : PROB a (prob_wreturn x) = 
-  PROB?.reflect (prob_return a x) *)
-
-(* let map_return (#a) (#b) (f:a->b) (x:a) : PROB b (prob_wreturn b (f x)) = 
-  PROB?.reflect (prob_return b (f x)) *)
-
-// let test2' () : PROB bool (fun p -> zero) = let c = coin () in c
-
+// Note that this one did not typecheck in ProbabilismWP without the simplifier
 let test3 x : PROB string (prob_wreturn x) = x
 
 let test4 () : PROB string (prob_wreturn "hello") = test3 "hello"
 
-let f (b:bool) : nat = if b then 0 else 1
-
-let goal = (ProbabilismHoare.prob_stronger (ProbabilismHoare.prob_wbind #Prims.bool
-             #Prims.nat
-             (fun pre post -> pre <=. (post true +. post false) /. FStar.Real.two)
-             (fun c -> ProbabilismHoare.prob_wreturn #Prims.nat (ProbabilismHoare.f c)))
-         (fun pre post -> pre <=. (post 0 +. post 1) /. FStar.Real.two))
-
-// let void #a (x:a) = ()
-
-(*let xx = assert_by_tactic (exists n. n=1) (fun () ->
-    witness (`2);
-    dump "Test";
-    admit_all()
-)*)
-
-irreducible
-let bind_return #a #b (wp1:prob_wp a) (f:a->b) : Lemma(prob_wbind wp1 (fun x -> prob_wreturn (f x)) 
-                                  == (fun pre post -> wp1 pre (fun x -> post (f x)))) =
-  admit()				     
-
-irreducible
-let return_bind #a #b (x:a) (wp2:a -> prob_wp b) : Lemma(prob_wbind (prob_wreturn x) wp2 == wp2 x) =
-  admit()
-
-irreducible
-let bind_simple_return #a #b wp1 f : Lemma(prob_wbind (simple_wp wp1) (fun x -> prob_wreturn (f x)) 
-                                  == simple_wp (fun post -> wp1 (fun x -> post (f x)))) =
-
-    assert (prob_wbind (simple_wp wp1) (fun x -> prob_wreturn (f x)) 
-        == simple_wp (fun post -> wp1 (fun x -> post (f x))))
-	by (
-	dump "x";
-	apply_lemma(`xxx);
-	admit_all()
-);
-
-()
-
-(*  
-  bind_return (simple_wp wp1) f;
-  assert (forall pre post. prob_wbind (simple_wp wp1) (fun x -> prob_wreturn (f x)) pre post
-       == simple_wp (fun post -> wp1 (fun x -> post (f x))) pre post);
-  admit();
-  ()				     
-
-(* let simple_wp #a (wp: prob_post a -> pr) : prob_wp a = fun pre post -> pre <=. wp post
- *)
-
-let test5 () : PROB nat (simple_wp (fun post -> (post 0 +. post 1) /. two)) by (
-unfold_def (`pure_null_wp);
-norm[];
-  dump "vc"
-) =
-  let c : bool = coin() in
-  f c
-
-(*
-
-// FAILS
-(* let test6 () : PROB nat (fun p -> (p 0 +. p 1) /. two) =
-  let c : bool = coin() in
-  map_return (fun c -> if c then 0 else 1) c *)
-
-// FAILS
-(* let test7 () : PROB nat (fun p -> (p 0 +. p 1) /. two) =
-  let c : bool = coin() in
-  f c *)
-
-let prob_unit : prob_wp unit = fun p -> p ()
-
-// FAILS
-(* let test7 () : PROB nat (fun p -> (p 0 +. p 1) /. two) =
-  let c : bool = coin() in
-  (if c then return 0 else return 1) *)
-
-let test8 () : PROB bool (fun post -> (post true +. post false) /. two) =
-  (if coin () then coin() else coin())
-
-
-let test7 () : PROB nat (fun p -> (p 0 +. p 1) /. two) =
-  let c : bool = coin() in
-  (if true then return 0 else return 1)
-
-// let reified = reify (test2 ())
-
-// let coin_vs_pick () : Lemma(coin () == pick [true;false]) = ()
-
+(* None of the tricky cases are included... *)
